theory/x64Semantics.thy
@@ -239,6 +239,7 @@ definition exec_instr :: "instruction \<Rightarrow> u64 \<Rightarrow> regset \<R
                          Some m' \<Rightarrow> Next (nextinstr_nf sz rs) m'))| 
   Paddl_rr  rd r1 \<Rightarrow> Next (nextinstr_nf sz (rs#(IR rd) <- (Val.add32 (rs (IR rd)) (rs (IR r1))))) m |
   Paddl_ri  rd n  \<Rightarrow> Next (nextinstr_nf sz (rs#(IR rd) <- (Val.add32 (rs (IR rd)) (Vint n)))) m |
+  Paddw_ri  rd n  \<Rightarrow> Next (nextinstr_nf sz (rs#(IR rd) <- (Val.add16 (rs (IR rd)) (Vshort n)))) m |
   Psubq_rr  rd r1 \<Rightarrow> Next (nextinstr_nf sz (rs#(IR rd) <- (Val.sub64 (rs (IR rd)) (rs (IR r1))))) m |
   Psubl_rr  rd r1 \<Rightarrow> Next (nextinstr_nf sz (rs#(IR rd) <- (Val.sub32 (rs (IR rd)) (rs (IR r1))))) m |
   Psubl_ri  rd n  \<Rightarrow> Next (nextinstr_nf sz (rs#(IR rd) <- (Val.sub32 (rs (IR rd)) (Vint n)))) m |
